define rope directly

Rope.dfy
@@ -1,15 +1,52 @@
-include "BinaryTree.dfy"
+include "Utils.dfy"
 
-module Rope {
-  import opened BinaryTree
-  type wbt = WeightedBinaryTree<string,nat>
+module BinaryTree {
+  import opened Utils
+  trait Node
+  {
+    var height: nat;
 
-  class Rope {
-    const rope: wbt
+    function length(): nat
+      reads this
+      decreases this.height
+  }
 
-    constructor (str: string)
+  class NTNode extends Node
+  {
+    var leftLen: nat;
+    var left: Node?;
+    var right: Node?;
+
+    constructor (left: Node, right: Node)
+      ensures this.leftLen == left.length()
+      ensures this.height > left.height
+      ensures this.height > right.height
     {
-      rope := wbt()
+      this.left := left;
+      this.right := right;
+      this.leftLen := left.length();
+      this.height := max(left.height, right.height) + 1;
     }
+
+    function length(): nat
+      reads this
+    {
+      this.leftLen + (if this.right == null then 0 else this.right.length())
+    }
+  }
+
+  class TNode extends Node
+  {
+    var str: string;
+
+    constructor(str: string)
+    {
+      this.str := str;
+      this.height := 1;
+    }
+
+    function length(): nat
+      reads this
+    { |this.str| }
   }
 }
