Utils.dfy
@@ -1,0 +1,17 @@
+module Utils {
+  function max(a: int, b: int): int
+    ensures max(a, b) >= a
+    ensures max(a, b) >= b
+    ensures max(a, b) == a || max(a, b) == b
+  {
+    if a >= b then a else b
+  }
+
+  function min(a: int, b: int): int
+    ensures min(a, b) <= a
+    ensures min(a, b) <= b
+    ensures min(a, b) == a || min(a, b) == b
+  {
+    if a <= b then a else b
+  }
+}
